Disjoint.v
@@ -7,7 +7,7 @@ From Elo Require Import Core.
 From Elo Require Import Access.
 From Elo Require Import Compat.
 From Elo Require Import AccessProp.
-From Elo Require Import NoLoc.
+From Elo Require Import Safe.
 
 Definition disjoint_memory m ths := forall tid1 tid2 ad,
   access m ths[tid1] ad ->
@@ -21,27 +21,21 @@ Local Lemma none_disjoint_memory_preservation : forall m m' ths t' tid,
   disjoint_memory m' ths[tid <- t'].
 Proof.
   intros * ? ? Hmstep tid1 tid2 ? ? ?. inversion Hmstep; subst.
-  destruct (Nat.eq_dec tid tid1), (Nat.eq_dec tid tid2); subst; eauto.
-  - rewrite (get_set_neq TM_Unit); rewrite (get_set_eq TM_Unit) in *;
-    eauto using mstep_none_inherits_access.
-  - rewrite (get_set_eq TM_Unit); rewrite (get_set_neq TM_Unit) in *;
-    eauto using mstep_none_preserves_not_access.
-  - rewrite (get_set_neq TM_Unit) in *; eauto.
+  destruct (Nat.eq_dec tid tid1), (Nat.eq_dec tid tid2); subst; eauto;
+  do 2 (rewrite_array TM_Unit);
+  eauto using mstep_none_inherits_access, mstep_none_preserves_not_access.
 Qed.
 
-Local Lemma load_disjoint_memory_preservation : forall m m' ths t' tid ad v,
+Local Lemma read_disjoint_memory_preservation : forall m m' ths t' tid ad v,
   disjoint_memory m ths ->
   tid < length ths ->
   m / ths[tid] ==[EF_Read ad v]==> m' / t' ->
   disjoint_memory m' ths[tid <- t'].
 Proof.
   intros * ? ? Hmstep tid1 tid2 ? ? ?. inversion Hmstep; subst.
-  destruct (Nat.eq_dec tid tid1), (Nat.eq_dec tid tid2); subst; eauto.
-  - rewrite (get_set_neq TM_Unit); rewrite (get_set_eq TM_Unit) in *;
-    eauto using mstep_load_inherits_access.
-  - rewrite (get_set_eq TM_Unit); rewrite (get_set_neq TM_Unit) in *;
-    eauto using mstep_load_preserves_not_access.
-  - rewrite (get_set_neq TM_Unit) in *; eauto.
+  destruct (Nat.eq_dec tid tid1), (Nat.eq_dec tid tid2); subst; eauto;
+  do 2 (rewrite_array TM_Unit);
+  eauto using mstep_read_inherits_access, mstep_read_preserves_not_access.
 Qed.
 
 Local Lemma alloc_disjoint_memory_preservation : forall m m' ths t' tid ad v,
@@ -56,40 +50,33 @@ Proof.
   { intros F. specialize (Hwba tid1 (length m) F). lia. }
   assert (~ access m (get TM_Unit ths tid2) (length m)).
   { intros F. specialize (Hwba tid2 (length m) F). lia. }
-  destruct (Nat.eq_dec tid tid1), (Nat.eq_dec tid tid2); subst; eauto.
-  - rewrite (get_set_neq TM_Unit); rewrite (get_set_eq TM_Unit) in *; eauto.
-    destruct (Nat.eq_dec ad' (length m)); subst;
-    eauto using inaccessible_address_add_2, mstep_alloc_inherits_access.
-  - rewrite (get_set_eq TM_Unit); rewrite (get_set_neq TM_Unit) in *; eauto.
-    destruct (Nat.eq_dec ad' (length m)); subst; eauto;
-    eauto using inaccessible_address_add_1, mstep_alloc_preserves_not_access.
-  - rewrite (get_set_neq TM_Unit) in *; eauto.
-    eauto using inaccessible_address_add_1, inaccessible_address_add_2.
+  destruct (Nat.eq_dec tid tid1), (Nat.eq_dec tid tid2); subst; eauto;
+  do 2 (rewrite_array TM_Unit);
+  eauto using inaccessible_address_add_1, inaccessible_address_add_2;
+  destruct (Nat.eq_dec ad' (length m)); subst;
+  eauto using inaccessible_address_add_1,
+              inaccessible_address_add_2,
+              mstep_alloc_inherits_access, 
+              mstep_alloc_preserves_not_access.
 Qed.
 
-Local Lemma store_disjoint_memory_preservation : forall m m' ths t' tid ad v,
+Local Lemma write_disjoint_memory_preservation : forall m m' ths t' tid ad v,
   disjoint_memory m ths ->
   tid < length ths ->
   m / ths[tid] ==[EF_Write ad v]==> m' / t' ->
   disjoint_memory m' ths[tid <- t'].
 Proof.
   intros * ? ? Hmstep tid1 tid2 ? ? ?. inversion Hmstep; subst.
-  destruct (Nat.eq_dec tid tid1), (Nat.eq_dec tid tid2); subst; eauto.
-  - rewrite (get_set_neq TM_Unit); rewrite (get_set_eq TM_Unit) in *;
-    eauto 6 using mstep_store_address_access,
-                  mstep_store_inherits_access,
-                  inaccessible_address_set_2.
-  - rewrite (get_set_eq TM_Unit); rewrite (get_set_neq TM_Unit) in *;
-    eauto 6 using mstep_store_address_access,
-                  mstep_store_preserves_not_access,
-                  inaccessible_address_set_1.
-  - rewrite (get_set_neq TM_Unit) in *;
-    eauto 8 using mstep_store_address_access,
-                  inaccessible_address_set_1,
-                  inaccessible_address_set_2.
+  destruct (Nat.eq_dec tid tid1), (Nat.eq_dec tid tid2); subst; eauto;
+  do 2 (rewrite_array TM_Unit);
+  eauto 8 using mstep_write_address_access,
+                mstep_write_inherits_access,
+                mstep_write_preserves_not_access,
+                inaccessible_address_set_1,
+                inaccessible_address_set_2.
 Qed.
 
-Local Lemma disjoint_memory_preservation' : forall m m' ths t' tid eff,
+Local Lemma mstep_disjoint_memory_preservation : forall m m' ths t' tid eff,
   (forall tid, valid_accesses m ths[tid]) ->
   disjoint_memory m ths ->
   tid < length ths ->
@@ -99,12 +86,12 @@ Proof.
   intros * ? ? ? Hmstep. inversion Hmstep; subst;
   eauto using none_disjoint_memory_preservation,
               alloc_disjoint_memory_preservation,
-              load_disjoint_memory_preservation,
-              store_disjoint_memory_preservation.
+              read_disjoint_memory_preservation,
+              write_disjoint_memory_preservation.
 Qed.
 
 Theorem disjoint_memory_preservation : forall m m' ths ths' tid eff,
-  threads_property SpawnNoLoc ths ->
+  threads_property SafeSpawns ths ->
   threads_property (valid_accesses m) ths ->
   disjoint_memory m ths ->
   tid < length ths ->
@@ -112,7 +99,7 @@ Theorem disjoint_memory_preservation : forall m m' ths ths' tid eff,
   disjoint_memory m' ths'.
 Proof.
   intros. inversion_cstep;
-  eauto using disjoint_memory_preservation'.
+  eauto using mstep_disjoint_memory_preservation.
   intros tid1 tid2 ad Hacc Hneq.
   decompose sum (lt_eq_lt_dec (length ths) tid2); subst.
   - rewrite (get_add_gt TM_Unit);
@@ -120,7 +107,8 @@ Proof.
     intros ?. inversion_access.
   - erewrite <- set_preserves_length.
     rewrite (get_add_eq TM_Unit).
-    eauto using noloc_for_block, noloc_then_not_access.
+    eauto using safe_for_block. (* safe_then_not_access *)
+    admit.
   - rewrite (get_add_lt TM_Unit);
     try solve [rewrite set_preserves_length; trivial].
     decompose sum (lt_eq_lt_dec (length ths) tid1); subst.
@@ -129,13 +117,16 @@ Proof.
       inversion_access.
     + erewrite <- set_preserves_length in Hacc.
       rewrite (get_add_eq TM_Unit) in Hacc.
+      (*
       assert (~ access m' block ad) by 
-        eauto using noloc_for_block, noloc_then_not_access.
+        eauto using safe_for_block, safe_then_not_access.
+      *)
       eauto.
+      admit.
     + rewrite (get_add_lt TM_Unit) in Hacc;
       try solve [rewrite set_preserves_length; trivial].
       destruct (Nat.eq_dec tid tid1), (Nat.eq_dec tid tid2); subst; eauto;
       do 2 (rewrite_array TM_Unit);
       eauto using step_spawn_inherits_access, step_spawn_preserves_not_access.
-Qed.
+Abort.
 
