Safe.v
@@ -1,0 +1,221 @@
+From Coq Require Import Arith.Arith.
+From Coq Require Import Lia.
+
+From Elo Require Import Util.
+From Elo Require Import Array.
+From Elo Require Import Core.
+From Elo Require Import Access.
+
+(* A term is safe if it has no mutable references. *)
+Inductive Safe : tm -> Prop :=
+  | safe_unit :
+    Safe <{ unit }> 
+
+  | safe_num : forall n,
+    Safe <{ N n }>
+
+  | safe_refI : forall ad T,
+    Safe <{ &ad :: i&T }>
+
+  | safe_new : forall T t,
+    Safe t ->
+    Safe <{ new T t }>
+
+  | safe_load : forall t,
+    Safe t ->
+    Safe <{ *t }>
+
+  | safe_asg : forall t1 t2,
+    Safe t1 ->
+    Safe t2 ->
+    Safe <{ t1 = t2 }>
+
+  | safe_id : forall x,
+    Safe <{ ID x }>
+
+  | safe_fun : forall x Tx t,
+    Safe t ->
+    Safe <{ fn x Tx --> t }>
+
+  | safe_call : forall t1 t2,
+    Safe t1 ->
+    Safe t2 ->
+    Safe <{ call t1 t2 }>
+
+  | safe_seq : forall t1 t2,
+    Safe t1 ->
+    Safe t2 ->
+    Safe <{ t1; t2 }>
+
+  | safe_spawn : forall t,
+    Safe t ->
+    Safe <{ spawn t }>
+  .
+
+(* A term has safe spawns if all its spawns are safe. *)
+Inductive SafeSpawns : tm -> Prop :=
+  | safe_spawns_unit :
+      SafeSpawns <{ unit }> 
+
+  | safe_spawns_num : forall n,
+      SafeSpawns <{ N n }>
+
+  | safe_spawns_ref : forall ad T,
+      SafeSpawns <{ &ad :: T }>
+
+  | safe_spawns_new : forall T t,
+      SafeSpawns t ->
+      SafeSpawns <{ new T t }>
+
+  | safe_spawns_load : forall t,
+      SafeSpawns t ->
+      SafeSpawns <{ *t }>
+
+  | safe_spawns_asg : forall t1 t2,
+      SafeSpawns t1 ->
+      SafeSpawns t2 ->
+      SafeSpawns <{ t1 = t2 }>
+
+  | safe_spawns_id : forall x,
+      SafeSpawns <{ ID x }>
+
+  | safe_spawns_fun : forall x Tx t,
+      SafeSpawns t ->
+      SafeSpawns <{ fn x Tx --> t }>
+
+  | safe_spawns_call : forall t1 t2,
+      SafeSpawns t1 ->
+      SafeSpawns t2 ->
+      SafeSpawns <{ call t1 t2 }>
+
+  | safe_spawns_seq : forall t1 t2,
+      SafeSpawns t1 ->
+      SafeSpawns t2 ->
+      SafeSpawns <{ t1; t2 }>
+
+  | safe_spawns_spawn : forall t,
+      Safe t ->
+      SafeSpawns <{ spawn t }>
+  .
+
+Local Ltac inversion_safe_spawns :=
+  match goal with
+  | H : SafeSpawns TM_Unit   |- _ => inversion H; subst; clear H
+  | H : SafeSpawns (_ _)     |- _ => inversion H; subst; clear H
+  | H : SafeSpawns (_ _ _)   |- _ => inversion H; subst; clear H
+  | H : SafeSpawns (_ _ _ _) |- _ => inversion H; subst; clear H
+  end.
+
+Local Lemma safe_spawns_subst : forall x Tx t t',
+  SafeSpawns <{ fn x Tx --> t }> ->
+  SafeSpawns t' ->
+  SafeSpawns ([x := t'] t).
+Proof.
+  intros * H ?. inversion_clear H;
+  induction t; eauto using SafeSpawns; simpl; 
+  try (destruct String.string_dec; trivial);
+  inversion_safe_spawns; eauto using SafeSpawns.
+Qed.
+
+Local Lemma safe_spawns_alloc : forall m t t' v,
+  SafeSpawns t ->
+  memory_property SafeSpawns m ->
+  t --[EF_Alloc (length m) v]--> t' ->
+  memory_property SafeSpawns (m +++ v).
+Proof.
+  intros. assert (SafeSpawns v).
+  { induction_step; inversion_safe_spawns; eauto. }
+  unfold memory_property. eauto using property_add, SafeSpawns.
+Qed.
+
+Local Lemma safe_spawns_store : forall m t t' ad v,
+  memory_property SafeSpawns m ->
+  SafeSpawns t ->
+  t --[EF_Write ad v]--> t' ->
+  memory_property SafeSpawns m[ad <- v].
+Proof.
+  intros. assert (SafeSpawns v).
+  { induction_step; inversion_safe_spawns; eauto. }
+  unfold memory_property. eauto using property_set, SafeSpawns.
+Qed.
+
+Local Lemma mstep_mem_safe_spawns_preservation : forall (m m' : mem) t t' eff,
+  memory_property SafeSpawns m ->
+  SafeSpawns t ->
+  m / t ==[eff]==> m' / t' ->
+  memory_property SafeSpawns m'.
+Proof.
+  intros. inversion_mstep; eauto using safe_spawns_alloc, safe_spawns_store.
+Qed.
+
+Local Lemma mstep_tm_safe_spawns_preservation : forall m m' t t' eff,
+  memory_property SafeSpawns m ->
+  SafeSpawns t ->
+  m / t ==[eff]==> m' / t' ->
+  SafeSpawns t'.
+Proof.
+  intros. inversion_mstep; induction_step; inversion_safe_spawns;
+  eauto using SafeSpawns, safe_spawns_subst.
+Qed.
+
+Local Lemma safe_then_safe_spawns : forall t,
+  Safe t ->
+  SafeSpawns t.
+Proof.
+  intros. induction t;
+  match goal with
+  | H : Safe _ |- _ =>
+    induction H; eauto using SafeSpawns
+  end.
+Qed.
+
+Local Lemma safe_spawns_for_block : forall t t' block,
+  SafeSpawns t ->
+  t --[EF_Spawn block]--> t' ->
+  SafeSpawns block.
+Proof.
+  intros. induction_step; inversion_safe_spawns;
+  eauto using SafeSpawns, safe_then_safe_spawns.
+Qed.
+
+Local Lemma step_safe_spawns_preservation : forall t t' block,
+  SafeSpawns t ->
+  t --[EF_Spawn block]--> t' ->
+  SafeSpawns t'.
+Proof.
+  intros. induction_step; inversion_safe_spawns;
+  eauto using SafeSpawns, safe_then_safe_spawns.
+Qed.
+
+Theorem safe_spawns_preservation : forall m m' ths ths' tid eff,
+  memory_property SafeSpawns m ->
+  threads_property SafeSpawns ths ->
+  m / ths ~~[tid, eff]~~> m' / ths' ->
+  (memory_property SafeSpawns m' /\ threads_property SafeSpawns ths').
+Proof.
+  intros. split; inversion_cstep;
+  eauto using mstep_mem_safe_spawns_preservation.
+  - eapply property_set; eauto using SafeSpawns.
+    eauto using mstep_tm_safe_spawns_preservation. (* performance *)
+  - eapply property_add; eauto using SafeSpawns, safe_spawns_for_block.
+    eapply property_set; eauto using SafeSpawns, step_safe_spawns_preservation.
+Qed.
+
+Lemma safe_for_block : forall t t' block,
+  SafeSpawns t ->
+  t --[EF_Spawn block]--> t' ->
+  Safe block.
+Proof.
+  intros. induction_step; inversion_safe_spawns; eauto.
+Qed.
+
+Lemma safe_then_not_access : forall m t ad,
+  Safe t ->
+  ~ access m t ad.
+Proof.
+  intros * Hsafe. induction t; inversion Hsafe; subst;
+  eapply not_access_iff; eauto using not_access.
+  eapply not_access_iff.
+  intros ?; inversion_access.
+Abort.
+
